[lf] wip on update_log_copy proof.

aneris/examples/reliable_communication/lib/repdb/resources/log_resources.v
@@ -2,15 +2,17 @@ From iris.algebra Require Import auth dfrac.
 From iris.algebra.lib Require Import mono_list.
 From iris.bi.lib Require Import fractional.
 From iris.proofmode Require Import tactics.
-From aneris.aneris_lang Require Import lang resources.
-
+From aneris.aneris_lang Require Import lang resources inject tactics proofmode.
+From aneris.aneris_lang.lib Require Import
+     list_proof monitor_proof lock_proof.
 
 (* ------------------------------------------------------------------------ *)
- Section Log_Resources_definition.
+ Section Logical_Log_Resources.
   Context `{!anerisG Mdl Σ}.
   Context {Aty : Type}.
   Notation A := (leibnizO Aty).
   Context `{inG Σ (mono_listUR A)}.
+
   (** Log resources. *)
 
 
@@ -41,4 +43,44 @@ From aneris.aneris_lang Require Import lang resources.
    naive_solver.
   Qed.
 
-End Log_Resources_definition.
+End Logical_Log_Resources.
+
+Section Physical_Log_Spec.
+  Context `{!anerisG Mdl Σ, !lockG Σ}.
+  Context {Aty : Type}.
+  Notation A := (leibnizO Aty).
+  Context `{inG Σ (mono_listUR A)}.
+  Context `{!Inject A val}.
+
+  Definition inject_log (xs : list A) :=
+    ($xs, #(List.length xs))%V.
+
+  Global Program Instance Inject_log `{!Inject A val}
+    : Inject (list A) val := {| inject := inject_log |}.
+  Next Obligation.
+    intros ? [] xs ys.
+    - inversion ys as [[Hinj Hinj2]].
+      symmetry. apply nil_length_inv. naive_solver.
+    - inversion ys as [[Hinj Hinj2]].
+      destruct xs as [| x xs]; first done.
+      simplify_eq.
+      inversion Hinj as [[Hinj3]]. apply Inject_list in Hinj3.
+      naive_solver.
+  Qed.
+
+  Definition is_log (logM : list A) (logV : val) :=
+    ∃ (lV : val), logV = (lV, #(List.length logM))%V ∧ is_list logM lV.
+
+  Definition log_monitor_inv_def
+    (ip : ip_address) (γlog : gname) (q: Qp)
+    (logL : loc) (Res : list A → iProp Σ) : iProp Σ :=
+    ∃ logV logM,
+      ⌜is_log logM logV⌝ ∗
+      logL ↦[ip] logV ∗
+      own_log_auth γlog q logM ∗
+      Res logM.
+
+  Definition log_monitor_inv monN ip monγ monV γlog q logL monR :=
+    is_monitor monN ip monγ monV (log_monitor_inv_def ip γlog q logL monR).
+
+End Physical_Log_Spec.
