aneris/examples/reliable_communication/lib/repdb/proof/leader/proof_of_update_log_copy_loop.v
@@ -1,0 +1,78 @@
+From iris.algebra.lib Require Import mono_list.
+From iris.base_logic Require Import invariants.
+From iris.bi.lib Require Import fractional.
+From iris.proofmode Require Import tactics coq_tactics reduction spec_patterns.
+From aneris.lib Require Import gen_heap_light.
+From aneris.aneris_lang Require Import lang resources inject tactics proofmode.
+From aneris.aneris_lang.lib Require Import list_proof monitor_proof lock_proof map_proof.
+From aneris.aneris_lang.lib.serialization Require Import serialization_proof.
+From aneris.aneris_lang.program_logic Require Import aneris_lifting.
+From aneris.aneris_lang.program_logic Require Import aneris_weakestpre.
+From aneris.examples.reliable_communication.prelude
+     Require Import ser_inj.
+From aneris.examples.reliable_communication.lib.mt_server
+     Require Import user_params mt_server_code.
+From aneris.examples.reliable_communication.lib.mt_server.spec
+     Require Import api_spec.
+From aneris.examples.reliable_communication.lib.repdb
+     Require Import repdb_code model.
+From aneris.examples.reliable_communication.lib.repdb.spec
+     Require Import db_params time events resources.
+From aneris.examples.reliable_communication.lib.repdb.resources
+     Require Import
+     ras log_resources resources_def
+     resources_global_inv resources_local_inv.
+From aneris.examples.reliable_communication.lib.repdb.proof
+     Require Import
+     repdb_serialization log_proof.
+From aneris.examples.reliable_communication.lib.repdb.proof.leader
+     Require Import
+     clients_mt_user_params.
+
+Import log_proof.
+
+Section UpdateLogCopy_Proof.
+  Context `{!anerisG Mdl Σ, dbparams : !DB_params, !IDBG Σ}.
+  Context (γL γM : gname).
+
+  Definition own_replog_loop γ l : iProp Σ :=
+    known_replog_token DB_addrF γ ∗ own_logL_obs γL l ∗ own_log_auth γ (1/4) l.
+
+  Lemma update_log_copy_loop_spec
+    (γF mFγ mCγ : gname) (kvsL logCL logFL : loc) (mvC mvF : val) :
+    {{{ leader_local_main_inv γL kvsL logCL mCγ mvC ∗
+       leader_local_secondary_inv γL logFL γF mFγ mvF ∗
+       own_replog_loop γF []
+    }}}
+      update_log_copy_loop #logCL mvC #logFL mvF #() @[ip_of_address DB_addr]
+    {{{ RET #(); True }}}.
+  Proof.
+    iIntros (Φ) "(#HinvL & #HinvF & Hloop) HΦ".
+    rewrite /update_log_copy_loop.
+    do 12 wp_pure _.
+    (* pose (@nil_length) as Hnl. *)
+    replace 0%Z with (Z.of_nat 0%nat); last done.
+    iAssert (⌜0%nat = List.length (@nil write_eventO)⌝)%I as "Hlen".
+    { done. }
+    iRevert "Hlen".
+    generalize 0%nat at 1 2 as m.
+    generalize (@nil write_eventO) as l.
+    iIntros (lF n Hlen).
+    iLöb as "IH" forall (lF n Hlen) "Hloop".
+    wp_pures.
+    wp_apply (monitor_acquire_spec with "[HinvL]"); first by iFrame "#".
+    iIntros (v) "( -> & Hlocked & Hres)".
+    wp_pures.
+    iDestruct "Hres" as (logV logM) "(Hlog & Hpl & HmainLog & HmainRes)".
+    wp_apply (wp_log_wait_until
+               with "[$HinvL $Hlocked $Hpl $HmainLog $Hlog $HmainRes][]").
+    admit.
+    iNext.
+    iIntros (logV' logM').
+    iIntros "(%Hlen' & %Hlog' & Hlocked & HmainRes & Hpl & HmainLog)".
+    wp_pures.
+    wp_load.
+    wp_pures.
+  Admitted.
+
+End UpdateLogCopy_Proof.
